seplogic: add more semantics work

Semantics.thy
@@ -32,40 +32,138 @@ fun trace_end :: \<open>'a trace \<Rightarrow> 'a\<close> where
 | \<open>trace_end (x \<cdot> TNil) = x\<close>
 | \<open>trace_end (_ \<cdot> a) = trace_end a\<close>
 
-subsection \<open> Trace Concat \<close>
+subsection \<open> Traces prefix ordered \<close>
 
-fun trace_concat :: \<open>'a trace \<Rightarrow> 'a trace \<Rightarrow> 'a trace\<close> (infixr \<open>@t\<close> 65) where
-  \<open>trace_concat TNil b = b\<close>
-| \<open>trace_concat (x \<cdot> a) b = x \<cdot> trace_concat a b\<close>
+instantiation trace :: (type) monoid_add
+begin
 
-lemma trace_concat_unit_right[simp]:
-  \<open>a @t TNil = a\<close>
+subsection \<open> trace plus \<close>
+
+definition \<open>zero_trace \<equiv> TNil\<close>
+
+(* concat *)
+fun plus_trace :: \<open>'a trace \<Rightarrow> 'a trace \<Rightarrow> 'a trace\<close> where
+  \<open>plus_trace TNil b = b\<close>
+| \<open>plus_trace (x \<cdot> a) b = x \<cdot> plus_trace a b\<close>
+
+lemma plus_trace_unit_right[simp]:
+  \<open>a + TNil = a\<close>
   by (induct a) simp+
 
-lemma trace_concat_assoc:
-  \<open>a @t b @t c = (a @t b) @t c\<close>
-  by (induct a arbitrary: b c) simp+
-
-lemma trace_start_concat[simp]:
-  \<open>trace_start (a @t b) = (if a = TNil then trace_start b else trace_start a)\<close>
+lemma trace_start_plus[simp]:
+  \<open>trace_start (a + b) = (if a = TNil then trace_start b else trace_start a)\<close>
   by (induct a arbitrary: b)
-    (force elim: trace_concat.elims)+
+    (force elim: plus_trace.elims)+
 
-lemma trace_end_concat[simp]:
-  \<open>trace_end (a @t b) = (if b = TNil then trace_end a else trace_end b)\<close>
+lemma trace_end_plus[simp]:
+  \<open>trace_end (a + b) = (if b = TNil then trace_end a else trace_end b)\<close>
   apply (induct a arbitrary: b)
    apply clarsimp
-  apply (case_tac \<open>a @t b\<close>)
-   apply (force elim: trace_concat.elims)
-  apply (simp, metis trace_concat_unit_right trace_end.simps(3))
+  apply (case_tac \<open>a + b\<close>)
+   apply (force elim: plus_trace.elims)
+  apply (simp, metis plus_trace_unit_right trace_end.simps(3))
   done
 
 lemma trace_concat_eq_nil_iff[simp]:
-  \<open>(a @t b) = TNil \<longleftrightarrow> a = TNil \<and> b = TNil\<close>
-  \<open>TNil = (a @t b) \<longleftrightarrow> a = TNil \<and> b = TNil\<close>
-  by (metis trace.discI trace_concat.elims)+
+  \<open>(a + b) = TNil \<longleftrightarrow> a = TNil \<and> b = TNil\<close>
+  \<open>TNil = (a + b) \<longleftrightarrow> a = TNil \<and> b = TNil\<close>
+  by (metis trace.discI plus_trace.elims)+
 
-subsection \<open> Parallel Trace Merge\<close>
+instance
+proof standard
+  fix a b c :: \<open>'a trace\<close>
+  show \<open>a + b + c = a + (b + c)\<close>
+    by (induct a arbitrary: b c) force+
+  show \<open>0 + a = a\<close>
+    by (simp add: zero_trace_def)
+  show \<open>a + 0 = a\<close>
+    by (simp add: zero_trace_def)
+qed
+
+end
+
+instantiation trace :: (type) order
+begin
+
+fun less_eq_trace :: \<open>'a trace \<Rightarrow> 'a trace \<Rightarrow> bool\<close> where
+  \<open>less_eq_trace (x \<cdot> a) (y \<cdot> b) = ((x = y) \<and> less_eq_trace a b)\<close>
+| \<open>less_eq_trace TNil _ = True\<close>
+| \<open>less_eq_trace _ _ = False\<close>
+
+lemma le_TNil_iff[simp]:
+  \<open>a \<le> TNil \<longleftrightarrow> a = TNil\<close>
+  using less_eq_trace.elims(1) by auto
+
+lemma le_TCons_iff:
+  \<open>a \<le> y \<cdot> b \<longleftrightarrow> a = TNil \<or> (\<exists>a'. a = y \<cdot> a' \<and> a' \<le> b)\<close>
+  using less_eq_trace.elims(2) by auto
+
+lemma TCons_le_iff[simp]:
+  \<open>x \<cdot> a \<le> b \<longleftrightarrow> (\<exists>b'. b = x \<cdot> b' \<and> a \<le> b')\<close>
+  using less_eq_trace.elims(2) by fastforce
+
+
+definition less_trace :: \<open>'a trace \<Rightarrow> 'a trace \<Rightarrow> bool\<close> where
+  \<open>less_trace a b \<equiv> a \<le> b \<and> \<not> (b \<le> a)\<close>
+
+instance
+proof standard
+  fix a b c :: \<open>'a trace\<close>
+  show \<open>(a < b) = (a \<le> b \<and> \<not> b \<le> a)\<close>
+    by (simp add: less_trace_def)
+  show \<open>a \<le> a\<close>
+    by (induct a) force+
+  show \<open>a \<le> b \<Longrightarrow> b \<le> c \<Longrightarrow> a \<le> c\<close>
+    apply (induct a b arbitrary: c rule: less_eq_trace.induct)
+      apply (metis less_eq_trace.simps(1,3) not_TNil_eq)
+     apply simp
+    apply simp
+    done
+  show \<open>a \<le> b \<Longrightarrow> b \<le> a \<Longrightarrow> a = b\<close>
+    by (induct a b rule: less_eq_trace.induct) force+
+qed
+
+end
+
+lemma trace_le_iff_add:
+  fixes a b :: \<open>'a trace\<close>
+  shows \<open>a \<le> b \<longleftrightarrow> (\<exists>c. b = a + c)\<close>
+  apply (induct b arbitrary: a)
+   apply simp
+  apply (case_tac a; force)
+  done
+
+instantiation trace :: (type) semilattice_inf
+begin
+
+fun inf_trace :: \<open>'a trace \<Rightarrow> 'a trace \<Rightarrow> 'a trace\<close> where
+  \<open>inf_trace (x \<cdot> a) (y \<cdot> b) = (if x = y then x \<cdot> (inf_trace a b) else TNil)\<close>
+| \<open>inf_trace _ _ = TNil\<close>
+
+lemma inf_trace_cons_left:
+  \<open>(x \<cdot> a) \<sqinter> b = (case b of TNil \<Rightarrow> TNil | y \<cdot> b' \<Rightarrow> if x = y then x \<cdot> (a \<sqinter> b') else TNil)\<close>
+  by (induct b arbitrary: a) force+
+
+lemma inf_trace_cons_right:
+  \<open>a \<sqinter> (y \<cdot> b) = (case a of TNil \<Rightarrow> TNil | x \<cdot> a' \<Rightarrow> if x = y then x \<cdot> (a' \<sqinter> b) else TNil)\<close>
+  by (induct a arbitrary: b) force+
+
+instance
+proof standard
+  fix a b c :: \<open>'a trace\<close>
+  show \<open>a \<sqinter> b \<le> a\<close>
+    by (induct b arbitrary: a)
+      (simp add: inf_trace_cons_right split: trace.splits)+
+  show \<open>a \<sqinter> b \<le> b\<close>
+    by (induct b arbitrary: a)
+      (simp add: inf_trace_cons_right split: trace.splits)+
+  show \<open>a \<le> b \<Longrightarrow> a \<le> c \<Longrightarrow> a \<le> b \<sqinter> c\<close>
+    by (induct a arbitrary: b c) force+
+qed
+
+end
+
+subsection \<open> Parallel Trace Merge \<close>
 
 inductive merge_traces_rel :: \<open>'a trace \<Rightarrow> 'a trace \<Rightarrow> 'a trace \<Rightarrow> bool\<close> where
   mergetr_nil: \<open>merge_traces_rel TNil TNil TNil\<close>
@@ -132,7 +230,7 @@ lemma merge_traces_assoc1:
     \<open>merge_traces_rel ab c abc\<close>
     \<open>a \<in> A\<close> \<open>b \<in> B\<close> \<open>c \<in> C\<close>
   shows
-    \<open>\<exists>a b c bc. a \<in> A \<and> b \<in> B \<and> c \<in> C \<and> merge_traces_rel b c bc \<and> merge_traces_rel a bc abc\<close>
+    \<open>\<exists>a\<in>A. \<exists>bc. (\<exists>b\<in>B. \<exists>c\<in>C. merge_traces_rel b c bc) \<and> merge_traces_rel a bc abc\<close>
   using assms
 proof (induct abc arbitrary: a b ab c A B C)
   case (TCons x abc)
@@ -179,7 +277,7 @@ lemma merge_traces_assoc2:
     \<open>merge_traces_rel a bc abc\<close>
     \<open>a \<in> A\<close> \<open>b \<in> B\<close> \<open>c \<in> C\<close>
   shows
-    \<open>\<exists>a b c ab. a \<in> A \<and> b \<in> B \<and> c \<in> C \<and> merge_traces_rel a b ab \<and> merge_traces_rel ab c abc\<close>
+    \<open>\<exists>ab. (\<exists>a\<in>A. \<exists>b\<in>B. merge_traces_rel a b ab) \<and> (\<exists>c\<in>C. merge_traces_rel ab c abc)\<close>
   using assms
 proof (induct abc arbitrary: a b c bc A B C)
   case (TCons x abc)
@@ -219,12 +317,13 @@ proof (induct abc arbitrary: a b c bc A B C)
 qed simp
 
 lemma merge_traces_rel_assoc:
-  \<open>{abc. \<exists>a. a \<in> A \<and> (\<exists>b. b \<in> B \<and> (\<exists>c. c \<in> C \<and> (\<exists>ab.
-      merge_traces_rel a b ab \<and> merge_traces_rel ab c abc)))}
-    = {abc. \<exists>a. a \<in> A \<and> (\<exists>b. b \<in> B \<and> (\<exists>c. c \<in> C \<and> (\<exists>bc.
-        merge_traces_rel b c bc \<and> merge_traces_rel a bc abc)))}\<close>
-  using merge_traces_assoc1 merge_traces_assoc2
-  by fast
+  \<open>{abc. \<exists>ab. (\<exists>a\<in>A. \<exists>b\<in>B. merge_traces_rel a b ab) \<and> (\<exists>c\<in>C. merge_traces_rel ab c abc)} =
+    {abc. \<exists>a\<in>A. \<exists>bc. (\<exists>b\<in>B. \<exists>c\<in>C. merge_traces_rel b c bc) \<and> merge_traces_rel a bc abc}\<close>
+  apply (clarsimp simp add: set_eq_iff)
+  apply (rule iffI)
+   apply (clarsimp, blast intro: merge_traces_assoc1)
+  apply (clarsimp, blast intro: merge_traces_assoc2)
+  done
 
 definition merge_traces :: \<open>'a trace \<Rightarrow> 'a trace \<Rightarrow> 'a trace set\<close> where
   \<open>merge_traces a b \<equiv> Collect (merge_traces_rel a b)\<close>
@@ -276,13 +375,6 @@ lemma TNil_merge_traces_TNil_parts:
   \<open>TNil \<in> merge_traces a b \<Longrightarrow> a = TNil \<or> b = TNil\<close>
   by (simp add: merge_traces_def)
 
-lemma merge_traces_assoc:
-  \<open>{abc|a b c ab abc::'a trace.
-      a \<in> A \<and> b \<in> B \<and> c \<in> C \<and> ab \<in> merge_traces a b \<and> abc \<in> merge_traces ab c}
-    = {abc|a b c bc abc.
-        a \<in> A \<and> b \<in> B \<and> c \<in> C \<and> bc \<in> merge_traces b c \<and> abc \<in> merge_traces a bc}\<close>
-  by (simp add: merge_traces_def merge_traces_rel_assoc)
-
 lemma merge_traces_rel_comm:
   \<open>merge_traces_rel a b c = merge_traces_rel b a c\<close>
   by (induct c arbitrary: a b)
@@ -297,40 +389,96 @@ lemma merge_traces_not_empty:
   by (induct a b rule: merge_traces_induct)
      (force simp add: merge_traces_def merge_traces_rel_cons_LR_iff)+
 
+definition
+  \<open>merge_trace_sets A B \<equiv> \<Union>a\<in>A. \<Union>b\<in>B. merge_traces a b\<close>
+
+lemma merge_trace_sets_assoc:
+  \<open>merge_trace_sets (merge_trace_sets A B) C = merge_trace_sets A (merge_trace_sets B C)\<close>
+  by (simp add: merge_trace_sets_def merge_traces_def Union_eq merge_traces_rel_assoc)
+
 section \<open>Processes\<close>
+
+subsection \<open> prefix closure \<close>
+
+definition \<open>prefixcl A \<equiv> {t. \<exists>t'\<in>A. t \<le> t'}\<close>
+
+lemma prefixcl_empty[simp]:
+  \<open>prefixcl {} = {}\<close>
+  by (simp add: prefixcl_def)
+
+lemma prefixcl_mono:
+  \<open>A \<le> B \<Longrightarrow> prefixcl A \<le> prefixcl B\<close>
+  by (force simp add: prefixcl_def)
+
+lemma prefixcl_increasing:
+  fixes A :: \<open>('a :: preorder) set\<close>
+  shows \<open>A \<le> prefixcl A\<close>
+  by (force simp add: prefixcl_def)
+
+lemma prefixcl_un[simp]:
+  \<open>prefixcl (A \<union> B) = prefixcl A \<union> prefixcl B\<close>
+  by (force simp add: prefixcl_def)
+
+lemma prefixcl_Union[simp]:
+  \<open>prefixcl (\<Union>\<A>) = \<Union>(prefixcl ` \<A>)\<close>
+  by (force simp add: prefixcl_def)
+
+
+lemma prefixcl_merge_traces[simp]:
+  \<open>prefixcl (merge_trace_sets A B) \<subseteq> merge_trace_sets (prefixcl A) (prefixcl B)\<close>
+  apply (clarsimp simp add: prefixcl_def merge_trace_sets_def merge_traces_def)
+  apply (rename_tac ab' a b ab)
+  sorry
+
+
+abbreviation (input) \<open>prefix_closed A \<equiv> prefixcl A \<subseteq> A\<close>
+
+lemma prefix_closed_strong:
+  fixes A :: \<open>('a :: preorder) set\<close>
+  shows \<open>prefix_closed A \<longleftrightarrow> prefixcl A = A\<close>
+  by (force simp add: prefixcl_def set_eq_iff subset_iff)
+
+subsection \<open> Typedef \<close>
 
 type_synonym 'a ptrace = \<open>('a pred \<times> 'a pred) trace\<close>
 
-datatype 'a process = Process (proctr: \<open>'a trace set\<close>)
+typedef 'a process = \<open>Collect prefix_closed :: 'a trace set set\<close>
+  morphisms proctr Process
+  by auto
+
+setup_lifting type_definition_process
 
 lemma process_eq_iff:
   \<open>a = b \<longleftrightarrow> proctr a = proctr b\<close>
-  using process.expand by auto
+  by (metis proctr_inverse)
 
 lemma eq_Process_iff_proctr_eq:
-  \<open>a = Process A \<longleftrightarrow> proctr a = A\<close>
-  by auto
+  \<open>prefix_closed A \<Longrightarrow> a = Process A \<longleftrightarrow> proctr a = A\<close>
+  by (metis Process_inverse mem_Collect_eq proctr_inverse)
 
 lemma Process_eq_iff_eq_proctr:
-  \<open>Process A = a \<longleftrightarrow> A = proctr a\<close>
-  by auto
+  \<open>prefix_closed A \<Longrightarrow> Process A = a \<longleftrightarrow> A = proctr a\<close>
+  by (metis Process_inverse mem_Collect_eq proctr_inverse)
 
 subsection \<open> Processes are a semiring \<close>
 
 instantiation process :: (type) comm_semiring_1
 begin
 
-definition plus_process :: \<open>'a process \<Rightarrow> 'a process \<Rightarrow> 'a process\<close> where
-  \<open>plus_process A B \<equiv> Process (proctr A \<union> proctr B)\<close>
+lift_definition plus_process :: \<open>'a process \<Rightarrow> 'a process \<Rightarrow> 'a process\<close> is
+  \<open>\<lambda>A B. A \<union> B\<close>
+  by (force simp add: prefixcl_def subset_iff)
 
-definition zero_process :: \<open>'a process\<close> where
-  \<open>zero_process \<equiv> Process {}\<close>
+lift_definition zero_process :: \<open>'a process\<close> is \<open>{}\<close>
+  by simp
 
-definition times_process :: \<open>'a process \<Rightarrow> 'a process \<Rightarrow> 'a process\<close> where
-  \<open>times_process A B \<equiv> Process (\<Union>(a,b) \<in> (proctr A \<times> proctr B). merge_traces a b)\<close>
+lift_definition times_process :: \<open>'a process \<Rightarrow> 'a process \<Rightarrow> 'a process\<close> is
+  \<open>\<lambda>A B. \<Union>(a,b) \<in> A\<times>B. merge_traces a b\<close>
+  apply clarsimp
+  sorry
 
-definition one_process :: \<open>'a process\<close> where
-  \<open>one_process \<equiv> Process {TNil}\<close>
+lift_definition one_process :: \<open>'a process\<close> is
+  \<open>{TNil}\<close>
 
 instance
 proof
@@ -368,7 +516,7 @@ instantiation process :: (type) monoid_seq
 begin
 
 definition seq_process :: \<open>'a process \<Rightarrow> 'a process \<Rightarrow> 'a process\<close> where
-  \<open>seq_process A B \<equiv> Process {a @t b|a b. a \<in> proctr A \<and> b \<in> proctr B}\<close>
+  \<open>seq_process A B \<equiv> Process {a + b|a b. a \<in> proctr A \<and> b \<in> proctr B}\<close>
 
 definition skip_process :: \<open>'a process\<close> where
   \<open>skip_process \<equiv> Process {TNil}\<close>
@@ -379,7 +527,7 @@ lemma process_skip_eq_one:
 
 instance
   apply standard
-    apply (simp add: seq_process_def set_eq_iff, metis trace_concat_assoc)
+    apply (simp add: seq_process_def set_eq_iff, metis (no_types) add.assoc)
    apply (simp add: seq_process_def skip_process_def)
   apply (simp add: seq_process_def skip_process_def)
   done
@@ -424,15 +572,19 @@ lemma process_inf_eq_plus: \<open>(a::'a process) \<sqinter> b = a + b\<close>
   by (simp add: inf_process_def plus_process_def)
 
 definition less_eq_process :: \<open>'a process \<Rightarrow> 'a process \<Rightarrow> bool\<close> where
-  \<open>less_eq_process a b \<equiv> proctr a \<supseteq> proctr b\<close>
+  \<open>less_eq_process a b \<equiv> prefixcl (proctr a) \<supseteq> prefixcl (proctr b)\<close>
 
 definition less_process :: \<open>'a process \<Rightarrow> 'a process \<Rightarrow> bool\<close> where
-  \<open>less_process a b \<equiv> proctr a \<supset> proctr b\<close>
+  \<open>less_process a b \<equiv> prefixcl (proctr a) \<supset> prefixcl (proctr b)\<close>
 
 instance
-  by standard
+  apply standard
+  apply
     (force simp add: less_process_def less_eq_process_def inf_process_def top_process_def
       process_eq_iff)+
+      apply (clarsimp simp add: less_process_def less_eq_process_def inf_process_def top_process_def
+      process_eq_iff)+
+  sledgehammer
 
 end
 
@@ -442,22 +594,6 @@ instance process :: (type) ordered_semiring_0
    apply (simp add: less_eq_process_def zero_process_def times_process_def)
   apply (simp add: less_eq_process_def zero_process_def times_process_def)
   done
-
-section \<open> Hoare Triples \<close>
-
-definition htriple' :: \<open>'a pred \<Rightarrow> ('a pred \<times> 'a pred) process \<Rightarrow> 'a pred \<Rightarrow> bool\<close>
-  (\<open>\<lbrace> _ \<rbrace> _ \<lbrace> _ \<rbrace>\<close> [0,0,0]) where
-  \<open>htriple' p a q \<equiv>
-    \<forall>t\<in>proctr a. if t = TNil then p \<le> q else snd (trace_end t) \<le> q\<close>
-
-lemma hoare_triple_ndet:
-  \<open>\<lbrace> p1 \<rbrace> a \<lbrace> q1 \<rbrace> \<Longrightarrow> \<lbrace> p2 \<rbrace> b \<lbrace> q2 \<rbrace> \<Longrightarrow> \<lbrace> p1 \<sqinter> p2 \<rbrace> a + b \<lbrace> q1 \<squnion> q2 \<rbrace>\<close>
-  by (force simp add: htriple'_def plus_process_def)
-
-lemma hoare_triple_seq:
-  \<open>\<lbrace> p \<rbrace> a \<lbrace> q \<rbrace> \<Longrightarrow> \<lbrace> q \<rbrace> b \<lbrace> r \<rbrace> \<Longrightarrow> \<lbrace> p \<rbrace> a \<triangleright> b \<lbrace> r \<rbrace>\<close>
-  by (force simp add: htriple'_def seq_process_def Ball_def all_conj_distrib
-      split: if_splits)
 
 section \<open> Specific Program Semantics \<close>
 
@@ -471,17 +607,97 @@ datatype ('x,'p) action =
   | AWritePtr 'p \<open>'p val\<close>
   | ASkip
   | AAbort
-  | ALocal \<open>('x \<rightharpoonup> 'p val) \<Rightarrow> ('x \<rightharpoonup> 'p val)\<close>
+  | ALocal \<open>(unit, 'x, 'p val) pheap \<Rightarrow> (unit, 'x, 'p val) pheap\<close>
 
 inductive sstep_sem ::
-  \<open>('x \<rightharpoonup> 'p val) \<times> ('p, 'p val) dheap \<Rightarrow> ('x,'p) action \<Rightarrow> ('x \<rightharpoonup> 'p val) \<times> ('p,'p val) dheap \<Rightarrow> bool\<close>
+  \<open>(unit, 'x, 'p val) pheap \<times> ('p, 'p val) dheap \<Rightarrow>
+    ('x,'p) action \<Rightarrow>
+    (unit, 'x, 'p val) pheap \<times> ('p,'p val) dheap \<Rightarrow>
+    bool\<close>
   (\<open>_ \<sim>_\<leadsto> _\<close> [51,0,51] 50 )
   where
   \<open>s \<sim>ASkip\<leadsto> s\<close>
-| \<open>h \<bullet>d p = None \<Longrightarrow> (l, h) \<sim>AAlloc x v\<leadsto> (l(x \<mapsto> VPtr p), h(p \<mapsto>d (full_perm, v)))\<close>
+| \<open>h \<bullet>d p = None \<Longrightarrow> (l, h) \<sim>AAlloc x v\<leadsto> (l(x \<mapsto>p ((), VPtr p)), h(p \<mapsto>d (full_perm, v)))\<close>
 | \<open>h \<bullet>d p = Some (full_perm, v) \<Longrightarrow> (l, h) \<sim>AFree p\<leadsto> (l, h |`d (-{p}))\<close>
-| \<open>h \<bullet>d p = Some (perm, v) \<Longrightarrow> (l, h) \<sim>AReadPtr p\<leadsto> (l(x \<mapsto> v), h)\<close>
+| \<open>h \<bullet>d p = Some (perm, v) \<Longrightarrow> (l, h) \<sim>AReadPtr x p\<leadsto> (l(x \<mapsto>p ((), v)), h)\<close>
 | \<open>h \<bullet>d p = Some (perm, v) \<Longrightarrow> wperm perm = 1 \<Longrightarrow> (l, h) \<sim>AWritePtr p v\<leadsto> (l, h(p \<mapsto>d (perm, v)))\<close>
 | \<open>(l, h) \<sim>ALocal f\<leadsto> (f l, h)\<close>
+
+inductive_cases sstep_sem_AFreeE[elim]: \<open>s \<sim>AFree p\<leadsto> s'\<close>
+
+lemma sstep_sem_AFree_iff:
+  \<open>(l,h) \<sim>AFree p\<leadsto> (l',h') \<longleftrightarrow> (l' = l \<and> h' = h |`d (- {p}) \<and> (\<exists>v. h \<bullet>d p = Some (full_perm, v)))\<close>
+  by (rule iffI; force intro: sstep_sem.intros)
+
+lemma sstep_sem_no_step_abort:
+  \<open>\<not> s \<sim>AAbort\<leadsto> s'\<close>
+proof -
+  { fix a
+  have  \<open>s \<sim>a\<leadsto> s' \<Longrightarrow> a = AAbort \<Longrightarrow> False\<close>
+    by (induct rule: sstep_sem.induct) simp+ }
+  then show ?thesis
+    by force
+qed
+
+section \<open> Unit pheap \<close>
+
+lemma unit_pheap_hperm_plus_eq:
+  fixes a b :: \<open>(unit, 'x, 'v) pheap\<close>
+  shows \<open>a \<bullet> x \<oplus>\<^sub>p b \<bullet> x =
+          (case b \<bullet> x of
+              None \<Rightarrow> a \<bullet> x
+            | Some (_, vb) \<Rightarrow>
+                (case a \<bullet> x of
+                  None \<Rightarrow> app_pheap b x
+                | Some (_, va) \<Rightarrow> Some ((), va)))\<close>
+  by (simp add: plus_hperm_def split: option.splits)
+
+section \<open> Hoare Triples \<close>
+
+definition htriple
+  :: \<open>('s::ord) pred \<Rightarrow>
+      ('s \<Rightarrow> 's \<Rightarrow> bool) \<Rightarrow>
+      's pred \<Rightarrow>
+      bool\<close>
+  (\<open>\<lbrace> _ \<rbrace> _ \<lbrace> _ \<rbrace>\<close> [0,0,0]) where
+  \<open>htriple p c q \<equiv> \<forall>s s'. c s s' \<longrightarrow> (\<exists>x. x \<le> s \<and> p x) \<longrightarrow> (\<exists>x. x \<le> s' \<and> q x)\<close>
+
+definition \<open>dealloc_cap p \<equiv> \<lambda>(l,h). \<exists>perm v. h \<bullet>d p = Some (perm, v) \<and> is_full_perm perm\<close>
+definition \<open>write_cap p \<equiv> \<lambda>(l,h). \<exists>perm v. h \<bullet>d p = Some (perm, v) \<and> is_write_perm perm\<close>
+
+lemma hoare_triple_ptr_write:
+  fixes P :: \<open>((unit, 'x, 'p val) pheap \<times> ('p, 'p val) dheap) pred\<close>
+  shows \<open>\<lbrace> dealloc_cap p \<rbrace> (\<lambda>s s'. s \<sim>AFree p\<leadsto> s') \<lbrace> emp \<rbrace>\<close>
+  apply (clarsimp simp add: htriple_def sstep_sem_AFree_iff sepconj_def dheap_eq_iff emp_def
+      dealloc_cap_def is_full_perm_def)
+  apply (metis Rep_dheap_zero app_zero_pheap sep_alg_class.zero_le)
+  done
+
+
+definition interp :: \<open>'a pred process \<Rightarrow> ('a \<Rightarrow> 'a \<Rightarrow> bool)\<close> where
+  \<open>interp p \<equiv> \<lambda>s s'.
+      (TNil \<in> proctr p \<longrightarrow> s = s') \<and>
+      (\<forall>t\<in>proctr p. t \<noteq> TNil \<longrightarrow> trace_start t s \<longrightarrow> trace_end t s')\<close>
+
+lemma hoare_triple_ndet:
+  fixes a b :: \<open>('a::ord) pred process\<close>
+  assumes
+    \<open>\<lbrace> p1 \<rbrace> interp a \<lbrace> q1 \<rbrace>\<close>
+    \<open>\<lbrace> p2 \<rbrace> interp b \<lbrace> q2 \<rbrace>\<close>
+  shows \<open>\<lbrace> p1 \<sqinter> p2 \<rbrace> interp (a + b) \<lbrace> q1 \<squnion> q2 \<rbrace>\<close>
+  using assms
+  by (auto simp add: htriple_def plus_process_def interp_def Ball_def all_conj_distrib
+      conj_disj_distribL ex_disj_distrib)
+
+lemma hoare_triple_seq:
+  fixes a b :: \<open>('a::ord) pred process\<close>
+  assumes
+    \<open>0 < a\<close>
+    \<open>\<lbrace> p \<rbrace> interp a \<lbrace> q \<rbrace>\<close>
+    \<open>\<lbrace> q \<rbrace> interp b \<lbrace> r \<rbrace>\<close>
+  shows \<open>\<lbrace> p \<rbrace> interp (a \<triangleright> b) \<lbrace> r \<rbrace>\<close>
+  using assms
+  by (clarsimp simp add: htriple_def seq_process_def interp_def leD less_eq_process_def
+      zero_process_def)
 
 end
