SepLogic.thy
@@ -751,38 +751,38 @@ begin
 
 definition plus_prod  :: \<open>'a \<times> 'b \<Rightarrow> 'a \<times> 'b \<Rightarrow> 'a \<times> 'b\<close> where
   \<open>plus_prod a b \<equiv> (fst a + fst b, snd a + snd b)\<close>
+declare plus_prod_def[simp]
 
 definition less_eq_prod  :: \<open>'a \<times> 'b \<Rightarrow> 'a \<times> 'b \<Rightarrow> bool\<close> where
   \<open>less_eq_prod a b \<equiv> (fst a \<le> fst b \<and> snd a \<le> snd b)\<close>
+declare less_eq_prod_def[simp]
 
 definition less_prod  :: \<open>'a \<times> 'b \<Rightarrow> 'a \<times> 'b \<Rightarrow> bool\<close> where
   \<open>less_prod x y \<equiv> fst x \<le> fst y \<and> snd x \<le> snd y \<and> (\<not> fst y \<le> fst x \<or> \<not> snd y \<le> snd x)\<close>
+declare less_prod_def[simp]
 
 definition disjoint_prod  :: \<open>'a \<times> 'b \<Rightarrow> 'a \<times> 'b \<Rightarrow> bool\<close> where
   \<open>disjoint_prod a b \<equiv> (fst a ## fst b \<and> snd a ## snd b)\<close>
+declare disjoint_prod_def[simp]
 
 definition zero_prod  :: \<open>'a \<times> 'b\<close> where
   \<open>zero_prod \<equiv> (0, 0)\<close>
+declare zero_prod_def[simp]
 
 definition bot_prod  :: \<open>'a \<times> 'b\<close> where
   \<open>bot_prod \<equiv> (\<bottom>, \<bottom>)\<close>
+declare bot_prod_def[simp]
 
 instance
   apply standard
-                apply (simp add: less_prod_def less_eq_prod_def)
-               apply (simp add: less_eq_prod_def)
-              apply (force simp add: less_eq_prod_def)
-             apply (force simp add: less_eq_prod_def)
-            apply (force simp add: bot_prod_def less_eq_prod_def)
-           apply (force simp add: zero_prod_def disjoint_prod_def)
-          apply (force simp add: zero_prod_def disjoint_prod_def)
-         apply (force simp add: disjoint_prod_def plus_prod_def partial_add_assoc)
-        apply (clarsimp simp add: disjoint_prod_def plus_prod_def, metis partial_add_commute)
-       apply (force simp add: disjoint_prod_def disjoint_symm)
-      apply (force simp add: disjoint_prod_def plus_prod_def dest: disjoint_add_rightL)
-     apply (force simp add: disjoint_prod_def plus_prod_def dest: disjoint_add_right_commute)
-    apply (force simp add: disjoint_prod_def plus_prod_def dest: positivity)
-   apply (clarsimp simp add: less_prod_def less_iff_sepadd plus_prod_def disjoint_prod_def)
+                apply force+
+         apply (force simp add: partial_add_assoc)
+        apply (force dest: partial_add_commute)
+       apply (force simp add: disjoint_symm)
+      apply (force dest: disjoint_add_rightL)
+     apply (force dest: disjoint_add_right_commute)
+    apply (force dest: positivity)
+   apply (clarsimp simp add: less_iff_sepadd)
     (* subgoal *)
    apply (rename_tac a1 b1 a2 b2)
    apply (case_tac \<open>a1 = a2\<close>)
@@ -791,7 +791,7 @@ instance
     apply (metis le_iff_sepadd order_class.order_eq_iff)
    apply (metis le_iff_sepadd order_class.order_eq_iff)
     (* done *)
-  apply (clarsimp simp add: plus_prod_def zero_prod_def)
+  apply force
   done
 
 end
@@ -801,9 +801,11 @@ begin
 
 definition plus_unit :: \<open>unit \<Rightarrow> unit \<Rightarrow> unit\<close> where
   \<open>plus_unit a b \<equiv> ()\<close>
+declare plus_unit_def[simp]
 
 definition disjoint_unit :: \<open>unit \<Rightarrow> unit \<Rightarrow> bool\<close> where
   \<open>disjoint_unit a b \<equiv> True\<close>
+declare disjoint_unit_def[simp]
 
 instance
   by standard simp+
